Use BufferNG as a transition from old to new buffers (WIP)

ulib/FStar.BufferNG.fst
@@ -1,18 +1,390 @@
-// with: --include ulib --include ulib/hyperstack
-
 module FStar.BufferNG
-module DM = FStar.DependentMap
 module HH = FStar.HyperHeap
 module HS = FStar.HyperStack
 module HST = FStar.HyperStack.ST
 module P = FStar.Pointer
-open FStar.Pointer
-open HST
 
-(* Buffers *)
+(* This module will help for the transition of some buffer-based code
+   It tries to sidestep the following two issues:
+   - the type of elements must be embeddable into P.typ
+   - all elements must always be readable (no uninitialized data)
+*)
 
-let buffer (t: typ): Tot Type0 = P.buffer t
+let rec supported
+  (t : P.typ)
+: Tot bool
+= match t with
+  | P.TBase _ -> true
+  | P.TStruct l -> struct_typ_supported l
+  | _ -> false
 
+and struct_typ_supported
+  (l: list (string * P.typ))
+: Tot bool
+= match l with
+  | [] -> true
+  | (_, t) :: l' -> supported t && struct_typ_supported l'
+
+let typ = (t: P.typ { supported t } )
+
+unfold
+let buffer
+  (t: typ)
+: Tot Type0
+= P.buffer t
+
+unfold
+let live (#a: typ) (h: HS.mem) (b: buffer a) : GTot Type0 = 
+  P.buffer_readable h b
+
+unfold
+let unused_in (#a: typ) (b: buffer a) (h: HS.mem) : GTot Type0 =
+  P.buffer_unused_in b h
+
+unfold
+let length (#a: typ) (b: buffer a) : GTot nat =
+  UInt32.v (P.buffer_length b)
+
+unfold
+let as_addr (#a: typ) (b: buffer a) : GTot nat =
+  P.buffer_as_addr b
+
+unfold
+let frameOf (#a: typ) (b: buffer a) : GTot HH.rid =
+  P.frameOf_buffer b
+
+unfold
+let as_seq (#a: typ) (h: HS.mem) (b: buffer a) : GTot (s: Seq.seq (P.type_of_typ a) { Seq.length s == length b } ) =
+  P.buffer_as_seq h b
+
+unfold
+let equal (#a: typ) (h: HS.mem) (b: buffer a) (h' : HS.mem) (b' : buffer a) : GTot Type0 =
+  as_seq h b == as_seq h' b'
+
+unfold
+let includes
+  (#a: typ)
+  (x y: buffer a)
+: GTot Type0
+= P.buffer_includes x y
+
+let includes_live
+  (#a: typ)
+  (h: HS.mem)
+  (x y : buffer a)
+: Lemma
+  (requires (x `includes` y /\ live h x))
+  (ensures (live h y))
+= P.buffer_includes_elim x y
+
+let includes_as_seq #a h1 h2 (x: buffer a) (y: buffer a)
+: Lemma
+  (requires (x `includes` y /\ as_seq h1 x == as_seq h2 x))
+  (ensures (as_seq h1 y == as_seq h2 y))
+= P.buffer_includes_elim x y
+
+let includes_trans #a (x y z: buffer a)
+: Lemma
+  (requires (x `includes` y /\ y `includes` z))
+  (ensures (x `includes` z))
+= P.buffer_includes_trans x y z
+
+unfold
+let disjoint (#a #a' : typ) (x: buffer a) (y: buffer a') : GTot Type0 =
+  P.loc_disjoint (P.loc_buffer x) (P.loc_buffer y)
+
+(* Disjointness is symmetric *)
+let lemma_disjoint_symm #a #a' (x:buffer a) (y:buffer a') : Lemma
+  (requires True)
+  (ensures (disjoint x y <==> disjoint y x))
+  [SMTPat (disjoint x y)]
+  = ()
+
+let lemma_disjoint_sub #a #a' (x:buffer a) (subx:buffer a) (y:buffer a') : Lemma
+  (requires (includes x subx /\ disjoint x y))
+  (ensures  (disjoint subx y))
+  [SMTPatT (disjoint subx y); SMTPatT (includes x subx)]
+  = P.buffer_includes_loc_includes x subx;
+    P.loc_disjoint_includes (P.loc_buffer x) (P.loc_buffer y) (P.loc_buffer subx) (P.loc_buffer y)
+
+let lemma_disjoint_sub' #a #a' (x:buffer a) (subx:buffer a) (y:buffer a') : Lemma
+  (requires (includes x subx /\ disjoint x y))
+  (ensures  (disjoint subx y))
+  [SMTPatT (disjoint y subx); SMTPatT (includes x subx)]
+  = ()
+
+let lemma_live_disjoint #a #a' h (b:buffer a) (b':buffer a') : Lemma
+  (requires (live h b /\ b' `unused_in` h))
+  (ensures (disjoint b b'))
+  [SMTPatT (disjoint b b'); SMTPatT (live h b)]
+= ()
+
+(** Concrete getters and setters *)
+val create
+  (#a:typ)
+  (init: P.type_of_typ a)
+  (len:UInt32.t)
+: HST.StackInline (buffer a)
+  (requires (fun h ->
+    UInt32.v len > 0
+  ))
+  (ensures (fun (h0: HS.mem) b h1 ->
+    UInt32.v len > 0 /\
+    b `unused_in` h0 /\
+    live h1 b /\
+    length b == UInt32.v len /\
+    frameOf b == h0.HS.tip /\
+    P.modifies_0 h0 h1 /\
+    as_seq h1 b == Seq.create (UInt32.v len) init
+  ))
+let create #a init len =
+  let len : P.array_length_t = len in
+  let content = P.screate (P.TArray len a) (Some (Seq.create (UInt32.v len) init)) in
+  P.buffer_of_array_pointer content
+
+unfold let p (#a:typ) (init:list (P.type_of_typ a)) : GTot Type0 =
+  normalize (0 < FStar.List.Tot.length init) /\
+  normalize (FStar.List.Tot.length init < UInt.max_int 32)
+
+unfold let q (#a:typ) (len:nat) (buf:buffer a) : GTot Type0 =
+  normalize (length buf == len)
+
+val createL
+  (#a: typ)
+  (init:list (P.type_of_typ a))
+: HST.StackInline (buffer a)
+  (requires (fun h -> p #a init))
+  (ensures (fun (h0: HS.mem) b h1 ->
+     let len = FStar.List.Tot.length init in
+     len > 0 /\
+     b `unused_in` h0 /\
+     live h1 b /\
+     length b == len /\
+     frameOf b == h0.HS.tip /\
+     P.modifies_0 h0 h1 /\
+     as_seq h1 b == Seq.of_list init /\
+     q #a len b
+   ))
+ 
+#set-options "--initial_fuel 1 --max_fuel 1" //the normalize_term (length init) in the pre-condition will be unfolded
+	                                     //whereas the L.length init below will not
+
+let createL #a init =
+  let len : P.array_length_t = UInt32.uint_to_t (List.Tot.length init) in
+  let s = Seq.of_list init in
+  Seq.lemma_of_list_length s init;
+  let content = P.screate (P.TArray len a) (Some s) in
+  P.buffer_of_array_pointer content
+
+#reset-options "--initial_fuel 0 --max_fuel 0"
+
+val rcreate
+  (#a: typ)
+  (r:HH.rid)
+  (init: P.type_of_typ a)
+  (len:UInt32.t)
+: HST.ST (buffer a)
+  (requires (fun h ->
+    HS.is_eternal_region r /\
+    UInt32.v len > 0
+  ))
+  (ensures (fun (h0: HS.mem) b h1 ->
+    b `unused_in` h0 /\
+    live h1 b /\
+    length b == UInt32.v len /\
+    h1.HS.tip == h0.HS.tip /\
+    P.modifies (P.loc_addresses r Set.empty) h0 h1 /\
+    as_seq h1 b == Seq.create (UInt32.v len) init
+  ))
+
+let rcreate #a r init len =
+  let len : P.array_length_t = len in
+  let content = P.ecreate (P.TArray len a) r (Some (Seq.create (UInt32.v len) init)) in
+  P.buffer_of_array_pointer content
+  
+val index
+  (#a: typ)
+  (b: buffer a)
+  (n: UInt32.t)
+: HST.Stack (P.type_of_typ a)
+  (requires (fun h ->
+    UInt32.v n < length b /\
+    live h b
+  ))
+  (ensures (fun h0 z h1 ->
+    UInt32.v n < length b /\
+    h1 == h0 /\
+    z == Seq.index (as_seq h0 b) (UInt32.v n)
+  ))
+
+let index #a b n =
+  P.read_buffer b n
+
+val upd
+  (#a: typ)
+  (b: buffer a)
+  (n: UInt32.t)
+  (z: P.type_of_typ a)
+: HST.Stack unit
+  (requires (fun h ->
+    live h b /\
+    UInt32.v n < length b
+  ))
+  (ensures (fun h0 _ h1 ->
+    live h1 b /\
+    UInt32.v n < length b /\
+    P.modifies (P.loc_pointer (P.gpointer_of_buffer_cell b n)) h0 h1 /\
+    as_seq h1 b == Seq.upd (as_seq h0 b) (UInt32.v n) z
+  ))
+
+let upd #a b n z =
+  let h0 = HST.get () in
+  P.write_buffer b n z;
+  let h1 = HST.get () in
+  assert (Seq.equal (as_seq h1 b) (Seq.upd (as_seq h0 b) (UInt32.v n) z))
+
+(* NOTE: Here I cannot fully respect the Buffer interface,
+   because pure sub no longer exists, since it has been split
+   into ghost gsub and stateful sub
+ *)
+
+unfold
+let gsub
+  (#a: typ)
+  (b: buffer a)
+  (i: UInt32.t)
+  (len: UInt32.t)
+: Ghost (buffer a)
+  (requires (UInt32.v i + UInt32.v len <= length b))
+  (ensures (fun _ -> True))
+= P.gsub_buffer b i len
+
+let sub
+  (#a: typ)
+  (b: buffer a)
+  (i: UInt32.t)
+  (len: UInt32.t)
+: HST.Stack (buffer a)
+  (requires (fun h ->
+    live h b /\
+    UInt32.v i + UInt32.v len <= length b
+  ))
+  (ensures (fun h0 b' h1 ->
+    live h0 b /\
+    UInt32.v i + UInt32.v len <= length b /\
+    h1 == h0 /\
+    b' == gsub b i len /\
+    b `includes` b'
+  ))
+= P.sub_buffer b i len
+
+let sub_sub
+  (#a: typ)
+  (b: buffer a)
+  (i1: UInt32.t)
+  (len1: UInt32.t)
+  (i2: UInt32.t)
+  (len2: UInt32.t)
+: Lemma
+  (requires (
+    UInt32.v i1 + UInt32.v len1 <= length b /\
+    UInt32.v i2 + UInt32.v len2 <= UInt32.v len1
+  ))
+  (ensures (
+    UInt32.v i1 + UInt32.v len1 <= length b /\
+    UInt32.v i2 + UInt32.v len2 <= UInt32.v len1 /\
+    gsub (gsub b i1 len1) i2 len2 == gsub b (UInt32.add i1 i2) len2
+  ))
+= ()  
+
+let sub_zero_length
+  (#a: typ)
+  (b: buffer a)
+: Lemma
+  (ensures (gsub b (UInt32.uint_to_t 0) (UInt32.uint_to_t (length b)) == b))
+= ()
+
+let lemma_sub_spec (#a:typ) (b:buffer a)
+  (i:UInt32.t)
+  (len:UInt32.t)
+  (h: HS.mem)
+: Lemma
+  (requires (
+    UInt32.v i + UInt32.v len <= length b /\
+    live h b
+  ))
+  (ensures  (
+    UInt32.v i + UInt32.v len <= length b /\
+    live h (gsub b i len) /\
+    as_seq h (gsub b i len) == Seq.slice (as_seq h b) (UInt32.v i) (UInt32.v i + UInt32.v len)
+  ))
+  [SMTPatOr [
+    [SMTPat (gsub b i len); SMTPatT (live h b)];
+    [SMTPat (live h (gsub b i len))]
+  ]]
+  = Seq.lemma_eq_intro (as_seq h (gsub b i len)) (Seq.slice (as_seq h b) (UInt32.v i) (UInt32.v i + UInt32.v len))
+
+(* Same here *)
+
+let goffset
+  (#a: typ)
+  (b: buffer a)
+  (i: UInt32.t)
+: Ghost (buffer a)
+  (requires (UInt32.v i <= length b))
+  (ensures (fun b' ->
+    UInt32.v i <= length b /\
+    b' == gsub b i (UInt32.sub (P.buffer_length b) i)
+  ))
+= P.gsub_buffer b i (UInt32.sub (P.buffer_length b) i)
+
+let offset
+  (#a:typ) 
+  (b:buffer a)
+  (i:UInt32.t)
+: HST.Stack (buffer a)
+  (requires (fun h0 ->
+    live h0 b /\
+    UInt32.v i <= length b
+  ))
+  (ensures (fun h0 b' h1 ->
+    h1 == h0 /\
+    UInt32.v i <= length b /\
+    b' == goffset b i
+  ))
+= P.offset_buffer b i
+
+let lemma_offset_spec
+  (#a: typ)
+  (b: buffer a)
+  (i: UInt32.t)
+  (h: HS.mem)
+: Lemma
+  (requires (
+    UInt32.v i <= length b /\
+    live h b
+  ))
+  (ensures (
+    UInt32.v i <= length b /\
+    as_seq h (goffset b i) == Seq.slice (as_seq h b) (UInt32.v i) (length b)
+  ))
+= ()
+
+
+
+
+
+
+(*
+  let content: reference (s:seq a{Seq.length s == v len}) =
+     salloc (Seq.create (v len) init) in
+  let b = MkBuffer len content 0ul len in
+  let h = HST.get() in
+  assert (Seq.equal (as_seq h b) (sel h b));
+  b
+
+
+(*
 let gsingleton_buffer_of_pointer
   (#t: typ)
   (p: pointer t)
